tools/Vale/src/ast.fs
@@ -65,6 +65,8 @@ type bindOp =
 | BindAlias // x @= eax (different from x := eax in treatment of old(x))
 | BindSet
 
+type tqual = TqExplicit | TqImplicit
+type cast = Upcast | Downcast
 type exp =
 | ELoc of loc * exp
 | EVar of id * typ option
@@ -74,9 +76,9 @@ type exp =
 | EBool of bool
 | EString of string
 | EOp of op * exp list * typ option
-| EApply of exp * typ list option * exp list * typ option
+| EApply of exp * (tqual * typ) list option * exp list * typ option
 | EBind of bindOp * exp list * formal list * triggers * exp * typ option
-| ECast of exp * typ
+| ECast of cast * exp * typ
 | ELabel of loc * exp // marker for exp that needs to be wrapped in a loc label
 
 and triggers = exp list list
@@ -96,7 +98,7 @@ type var_storage =
 | XAlias of var_alias * exp // variable is a name for some other storage
 | XState of exp // top-level declaration of member of the state (e.g. a register)
 
-type assert_attrs = {is_inv:bool; is_split:bool; is_refined:bool; is_quicktype:bool}
+type assert_attrs = {is_inv:bool; is_split:bool; is_refined:bool; is_quicktype:bool option}
 type quick_info = {qsym:string; qmods:id list}
 type lhs = id * (typ option * ghost) option // TODO: we only allow Ghost here, so no need to mention possibility of NotGhost; can just be id * formal option
 type stmt =
